> নিচের প্রায় সবগুলো উত্তরই LLM generated, তবে যদি কোনোটা নিয়ে সংশয় সৃষ্টি হয়, feel free to ask!
## Equivalence Check

> একটা কথা মাথায় রাখতে হবে যে $\models$ এই চিহ্নটা হলো logical entails, বাম পাশে সত্য আর ডান পাশে মিথ্যা এরকম কখনোই হতে পারবে না ;)

> আর == এটা হলো equivalence যেটা আমরা `tpointtech` এ পড়েছি 

### i. $(A \land B) \models (A \Leftrightarrow B)$

**This statement is correct.**

- **Clarification:** The symbol $\models$ means "logically entails." This statement asserts that in every situation where $(A \land B)$ is true, $(A \Leftrightarrow B)$ must also be true.
    
    - For $(A \land B)$ to be true, both **A** and **B** must be true.
        
    - The expression $(A \Leftrightarrow B)$ is true if and only if **A** and **B** have the same truth value.
        
    - Therefore, in the specific case where both **A** and **B** are true, $(A \Leftrightarrow B)$ is also true. This confirms the entailment.
        
    
    We can also see this with a truth table:
    

| **A** | **B** | **A∧B** | **A⇔B** |
| ----- | ----- | ------- | ------- |
| T     | T     | **T**   | **T**   |
| T     | F     | F       | F       |
| F     | T     | F       | F       |
| F     | F     | F       | T       |

The only row where $(A \land B)$ is true is the first row, and in that row, $(A \Leftrightarrow B)$ is also true.

---

### ii. $A \Leftrightarrow B \models \neg A \lor B$

**This statement is correct.**

- **Clarification:** We need to check if $\neg A \lor B$ is true in all cases where $A \Leftrightarrow B$ is true.
    
    - $A \Leftrightarrow B$ is true under two conditions:
        
        1. Both A and B are true.
            
        2. Both A and B are false.
            
    - Let's check the expression $\neg A \lor B$ (which is equivalent to $A \Rightarrow B$) for these two conditions:
        
        1. If A=True and B=True, then $\neg T \lor T \Rightarrow F \lor T$, which is **True**.
            
        2. If A=False and B=False, then $\neg F \lor F \Rightarrow T \lor F$, which is **True**.
            
    - Since $\neg A \lor B$ is true in all cases where $A \Leftrightarrow B$ is true, the entailment holds.
        

---

### iii. $(A \lor B) \land (\neg C \lor \neg D \lor E) \models (A \lor B \lor C) \land (B \land C \land D \Rightarrow E)$

**This statement is correct.**

- **Clarification:** Let the left-hand side (LHS) be our premises and the right-hand side (RHS) be our conclusion. The LHS gives us two premises:
    
    1. $P_1: (A \lor B)$
        
    2. $P_2: (\neg C \lor \neg D \lor E)$
        
    
    The RHS is a conjunction, so we must be able to derive both parts from the premises.
    
    - **Part 1 of RHS:** $(A \lor B \lor C)$
        
        - We can derive this directly from $P_1$ using the **Rule of Addition** (or Disjunction Introduction), which states that if we have $P$, we can infer $P \lor Q$. Since we have $(A \lor B)$, we can validly infer $(A \lor B) \lor C$.
            
    - **Part 2 of RHS:** $(B \land C \land D \Rightarrow E)$
        
        - First, convert the implication to its equivalent disjunctive form: $\neg(B \land C \land D) \lor E$, which simplifies to $(\neg B \lor \neg C \lor \neg D \lor E)$ using De Morgan's laws.
            
        - We can derive this from $P_2$ using the **Rule of Addition**. Since we have $(\neg C \lor \neg D \lor E)$, we can validly infer $\neg B \lor (\neg C \lor \neg D \lor E)$.
            
    
    Since both parts of the RHS conclusion can be logically derived from the LHS premises, the entire statement is correct.
    

---

### iv. $(A \land B) \Rightarrow C \models (A \Rightarrow C) \lor (B \Rightarrow C)$

**This statement is correct.**

- **Clarification:** This is a case of logical equivalence. If two expressions are logically equivalent, they also entail each other. We can prove this by converting both sides into a standard form.
    
    - **Left-Hand Side (LHS):** $(A \land B) \Rightarrow C$
        
        - $\equiv \neg(A \land B) \lor C$ (Implication Equivalence)
            
        - $\equiv (\neg A \lor \neg B) \lor C$ (De Morgan's Law)
            
        - $\equiv \neg A \lor \neg B \lor C$
            
    - **Right-Hand Side (RHS):** $(A \Rightarrow C) \lor (B \Rightarrow C)$
        
        - $\equiv (\neg A \lor C) \lor (\neg B \lor C)$ (Implication Equivalence)
            
        - $\equiv \neg A \lor C \lor \neg B \lor C$
            
        - $\equiv \neg A \lor \neg B \lor C$ (by Idempotent Law, where $C \lor C \equiv C$)
            
    
    Since both the LHS and RHS simplify to the exact same logical expression $(\neg A \lor \neg B \lor C)$, they are logically equivalent, and the entailment is correct.
    

---
### v. $A \Leftrightarrow B \models A \lor B$

❌ **Incorrect.**

- **Reasoning:** The entailment fails when **A** and **B** are both false.
    
    - If A=False and B=False, then $(A \Leftrightarrow B)$ is **true**.
        
    - However, $(A \lor B)$ becomes $(F \lor F)$, which is **false**.
        
    - Since we found a case where the premise is true but the conclusion is false, the statement is incorrect.
        

---

### vi. $A \Rightarrow B \models \neg A \lor B$

✅ **Correct.**

- **Reasoning:** This is a fundamental logical equivalence. The expression $A \Rightarrow B$ (A implies B) is defined as being logically equivalent to $\neg A \lor B$. Since they are equivalent, they entail each other.
    

---

### iv. $(A \lor B) \land (\neg C \lor \neg D \lor E) \models (A \lor B \lor C) \land (B \land C \land D \Rightarrow E)$

✅ **Correct.**

- **Reasoning:** Both parts of the conclusion on the right side can be logically derived from the premises on the left side using the **Rule of Addition**, which allows you to add any proposition to an existing one with an 'OR' operator. For example, since we know $(A \lor B)$ is true, we can infer that $(A \lor B \lor C)$ must also be true.
    

---

### v. $(A \lor B) \land (\neg C \lor \neg D \lor E) \models (A \lor B) \land (\neg D \lor E)$

❌ **Incorrect.**

- **Reasoning:** This statement claims that if $(\neg C \lor \neg D \lor E)$ is true, then $(\neg D \lor E)$ must also be true. This is not valid.
    
    - **Counterexample:** Let C=False, D=True, and E=False.
        
    - The premise $(\neg C \lor \neg D \lor E)$ becomes $(T \lor F \lor F)$, which is **true**.
        
    - However, the conclusion $(\neg D \lor E)$ becomes $(F \lor F)$, which is **false**.
        

---

### vi. $(A \lor B) \land \neg(A \Rightarrow B)$ is satisfiable

✅ **Correct.**

- **Reasoning:** An expression is **satisfiable** if there's at least one assignment of truth values that makes it true. Let's simplify the expression:
    
    - $(A \lor B) \land \neg(\neg A \lor B)$
        
    - $(A \lor B) \land (A \land \neg B)$ (Using De Morgan's Law)
        
- For this entire expression to be true, the part $(A \land \neg B)$ must be true, which means **A must be True** and **B must be False**.
    
- This assignment (A=T, B=F) makes the entire expression true, so it is satisfiable.
    

---

### vii. $(A \land B) \Rightarrow C \models (A \Rightarrow C) \lor (B \Rightarrow C)$

✅ **Correct.**

- **Reasoning:** The expressions on the left and right are logically equivalent. Both can be simplified to the same form: $\neg A \lor \neg B \lor C$. Since they are equivalent, the entailment is correct.
    

## First Order Logic 
### A. Every cat loves its mother or father.

- **(i) ∀x Cat(x) ⇒ Loves(x, Mother(x) v Father(x))**
    
    - **(2) Syntactically invalid.** The arguments to a predicate like `Loves` must be terms (variables, constants, or functions). The expression `Mother(x) v Father(x)` is a logical disjunction, not a term. You cannot "love" a logical "or".
        
- **(ii) ∀x ¬Cat(x) v Loves(x, Mother(x)) v Loves(x, Father(x))**
    
    - **(1) Correctly expresses the sentence.** This is logically equivalent to the standard form `∀x Cat(x) ⇒ (Loves(x, Mother(x)) v Loves(x, Father(x)))`. The equivalence rule used here is that `P ⇒ Q` is the same as `¬P v Q`.
        
- **(iii) ∀x Cat(x) ∧ (Loves(x, Mother(x)) v Loves(x, Father(x)))**
    
    - This expression is syntactically valid, but it **does not correctly express the sentence**. It claims that everything in the universe is a cat (`∀x Cat(x)`), which is incorrect. The proper logical connective to use with a universal quantifier (`∀`) for "Every..." statements is implication (`⇒`), not conjunction (`∧`).
        

---

### B. Every dog who loves one of its brothers is happy.

- **(i) ∀x Dog(x) ∧ (∃y Brother(y, x) ∧ Loves(x, y)) ⇒ Happy(x)**
    
    - **(2) Syntactically invalid.** The scope of the universal quantifier `∀x` is not correctly applied to the entire sentence. As written, the `x` in `Happy(x)` is a "free variable" because it's outside the scope of `∀x`. The entire expression should be enclosed in brackets after the `∀x`.
        
- **(ii) ∀x [Dog(x) ∧ (∃y Brother(y, x) ∧ Loves(x, y))] ⇒ Happy(x)**
    
    - **(1) Correctly expresses the sentence.** This translates to: "For any x, if x is a dog AND there exists a y such that y is a brother of x AND x loves y, THEN x is happy." This perfectly captures the sentence's meaning.
        
- **(iii) ∀x Dog(x) ∧ [∀y Brother(y, x) ⇒ Loves(x, y)] ⇒ Happy(x)**
    
    - **(2) Syntactically invalid.** This has the same scope issue as expression (i), where the `x` in `Happy(x)` is a free variable. Additionally, it incorrectly uses a universal quantifier (`∀y`), which would mean the dog loves **all** of its brothers, not just **one** of them.
        

---

### C. No dog bites a child of its owner.

- **(i) ∀x Dog(x) ⇒ ¬Bites(x, Child(Owner(x)))**
    
    - **(2) Syntactically invalid.** The expression `Child(Owner(x))` is being used as a function that returns a single object ("the child"), but the original sentence implies any child. Logic requires a predicate `Child(y, z)` (y is a child of z) and a quantifier for the child (`y`).
        
- **(ii) ¬∃x, y Dog(x) ∧ Child(y, Owner(x)) ∧ Bites(x, y)**
    
    - **(1) Correctly expresses the sentence.** This reads: "There does not exist an x and a y such that x is a dog, y is a child of x's owner, and x bites y." This is an accurate way to state the original sentence.
        
- **(iii) ∀x Dog(x) ⇒ (∀y Child(y, Owner(x)) ⇒ ¬Bites(x, y))**
    
    - **(1) Correctly expresses the sentence.** This is a logically equivalent and correct formulation. It reads: "For any x, if x is a dog, then for any y, if y is a child of x's owner, then x does not bite y."
        
- **(iv) ¬∃x Dog(x) ⇒ (∃y Child(y, Owner(x)) ∧ Bites(x, y))**
    
    - **(2) Syntactically invalid.** The scope of `¬∃x` only covers `Dog(x)`. The variables `x` that appear later in the expression (`Owner(x)` and `Bites(x, y)`) are free and not bound by any quantifier.
        

---

### D. Everyone's zip code within a state has the same first digit.

- **(i) ∀x, s, z1 [State(s) ∧ LivesIn(x, s) ∧ Zip(x)=z1] ⇒ [∀y, z2 LivesIn(y, s) ∧ Zip(y)=z2 ⇒ Digit(1, z1)=Digit(1, z2)]**
    
    - **(1) Correctly expresses the sentence.** Although it's written in a complex way by introducing `z1` and `z2` to represent the zip codes, it is logically sound. It states that for any person `x` in a state `s` with zip `z1`, any other person `y` in the same state with zip `z2` will have the same first digit.
        
- **(ii) ∀x, s [State(s) ∧ LivesIn(x, s) ∧ ∃z1 Zip(x)=z1] ⇒ [∀y, z2 LivesIn(y, s) ∧ Zip(y)=z2 ∧ Digit(1, z1)=Digit(1, z2)]**
    
    - **(2) Syntactically invalid.** The variable `z1` is introduced with an existential quantifier (`∃z1`) in the antecedent (the `if` part), but it is then used in the consequent (the `then` part). A variable's scope does not extend outside of the clause where its quantifier is located.
        
- **(iii) ∀x, y, s State(s) ∧ LivesIn(x, s) ∧ LivesIn(y, s) ⇒ Digit(1, Zip(x)=Zip(y))**
    
    - **(2) Syntactically invalid.** The function `Digit(...)` expects a zip code as its second argument. The expression `Zip(x)=Zip(y)` is a logical comparison that evaluates to true or false; it is not a zip code and cannot be an argument for the `Digit` function.
        
- **(iv) ∀x, y, s (State(s) ∧ LivesIn(x, s) ∧ LivesIn(y, s)) ⇒ Digit(1, Zip(x))=Digit(1, Zip(y))**
    
    - **(1) Correctly expresses the sentence.** This is the most clear and direct translation. It says: "For any two people x and y and any state s, if s is a state and both x and y live in s, then the first digit of x's zip code is equal to the first digit of y's zip code."
        


## First order Logic - Translation
### 📝 Predicate Definitions

প্রশ্ন উত্তরে সুবিধার্থে কিছু function ব্যবহার করা যেতে পারে, এটা optional, যার যেভাবে খুশি ধরে নেয়া যাবে...

- **Gardener(x)**: $x$ is a gardener.
    
- **Likes(x, y)**: $x$ likes $y$.
    
- **TheSun**: A constant representing the sun.
    
- **Person(x)**: $x$ is a person.
    
- **Time(t)**: $t$ is a time.
    
- **CanFool(x, t)**: Person $x$ can be fooled at time $t$.
    
- **Mushroom(x)**: $x$ is a mushroom.
    
- **Purple(x)**: $x$ is purple.
    
- **Poisonous(x)**: $x$ is poisonous.
    
- **Clinton**: A constant representing Clinton.
    
- **Tall(x)**: $x$ is tall.
    
- **Man(x)**: $x$ is a man.
    
- **Fool(x)**: $x$ is a fool.
    
- `Surgeon(x)`: $x$ is a surgeon.
	
- `Lawyer(x)`: $x$ is a lawyer.
	
- `Actor(x)`: $x$ is an actor.
	
- `Doctor(x)`: $x$ is a doctor.
	
- `HoldsAnotherJob(x)`: $x$ holds a job in addition to one already mentioned.
	
- `BossOf(x, y)`: $x$ is the boss of $y$.
	
- `CustomerOf(x, y)`: $x$ is a customer of $y$.
        

---

### Set - I

**i. Every gardener likes the sun.**

- **Answer:** $∀x (Gardener(x) → Likes(x, TheSun))$
    

**ii. You can fool some of the people all of the time.**

- **Answer:** $∃x (Person(x) ∧ ∀t (Time(t) → CanFool(x, t)))$
    

**iii. You can fool all of the people some of the time.**

- **Answer:** $∀x (Person(x) → ∃t (Time(t) ∧ CanFool(x, t)))$
    

**iv. All purple mushrooms are poisonous.**

- **Answer:** $∀x ((Mushroom(x) ∧ Purple(x)) → Poisonous(x))$
    

**v. No purple mushroom is poisonous.**

- **Answer:** $∀x ((Mushroom(x) ∧ Purple(x)) → ¬Poisonous(x))$
    

**vi. There are exactly two purple mushrooms.**

- **Answer:** $∃x ∃y ( (Mushroom(x) ∧ Purple(x)) ∧ (Mushroom(y) ∧ Purple(y)) ∧ (x ≠ y) ∧ ∀z ((Mushroom(z) ∧ Purple(z)) → (z=x ∨ z=y)) )$
    

**vii. Clinton is not tall.**

- **Answer:** $¬Tall(Clinton)$
    

**viii. All men are not fool.**

- **Answer:** $∃x (Man(x) ∧ ¬Fool(x))$
    
    > **Note:** This translation assumes the sentence means "Not all men are fools." The English is slightly ambiguous. If it were to mean "No man is a fool," the translation would be $∀x (Man(x) → ¬Fool(x))$.
    

---

### Set - II

**i. Emily is either a surgeon or a lawyer.**

- **Answer:** `Surgeon(Emily) ∨ Lawyer(Emily)`
    

**ii. Joe is an actor, but he also holds another job.**

- **Answer:** `Actor(Joe) ∧ HoldsAnotherJob(Joe)`
    
    > **Note:** "But" is translated as a logical AND (`∧`). The concept of "another job" is represented with a dedicated predicate for simplicity.
    

**iii. All surgeons are doctors.**

- **Answer:** $∀x (Surgeon(x) → Doctor(x))$
    

**iv. Joe does not have a lawyer (i.e., is not a customer of any lawyer).**

- **Answer:** $¬∃x (Lawyer(x) ∧ CustomerOf(Joe, x))$
    
    - This can also be written equivalently as: $∀x (Lawyer(x) → ¬CustomerOf(Joe, x))$
        

**v. Emily has a boss who is a lawyer.**

- **Answer:** $∃x (BossOf(x, Emily) ∧ Lawyer(x))$
    

**vi. There exists a lawyer all of whose customers are doctors.**

- **Answer:** $∃x (Lawyer(x) ∧ ∀y (CustomerOf(y, x) → Doctor(y)))$
    

**vii. Every surgeon has a lawyer.**

- **Answer:** $∀x (Surgeon(x) → ∃y (Lawyer(y) ∧ CustomerOf(x, y)))$
    

